Program-proofs/Exercises/Invariants/prob19/prob19.dfy
@@ -3,6 +3,9 @@
    description: extra practice in Dafny, invariants, prob19
 */
 
+include "../../CommonSupport.dfy"
+import opened CommonFunctions
+
 method problem19(a: array<int>) returns (r: int)
 requires ??
 ensures  ??
@@ -17,7 +20,8 @@ ensures  ??
         
         {P: n > 0}
       T
-        {Q: r = Max (a[i] + a[j] + a[h] | i,j,h: 0 ≤ i ≤ j < n ∧ i ≤ h < n)}
+        {Q: r = Max (a[i] + a[j] + a[h] 
+                     | i,j,h: 0 ≤ i ≤ j < n ∧ i ≤ h < n)}
 
     The time complexity of T should be linear in n.
   */
